@prefix : <http://purl.obolibrary.org/obo/foodon/imports/robot_wine.owl#> .
@prefix owl: <http://www.w3.org/2002/07/owl#> .
@prefix rdf: <http://www.w3.org/1999/02/22-rdf-syntax-ns#> .
@prefix xml: <http://www.w3.org/XML/1998/namespace> .
@prefix xsd: <http://www.w3.org/2001/XMLSchema#> .
@prefix rdfs: <http://www.w3.org/2000/01/rdf-schema#> .
@base <http://purl.obolibrary.org/obo/foodon/imports/robot_wine.owl> .

<http://purl.obolibrary.org/obo/foodon/imports/robot_wine.owl> rdf:type owl:Ontology .

#################################################################
#    Annotation properties
#################################################################

###  http://purl.obolibrary.org/obo/IAO_0000114
<http://purl.obolibrary.org/obo/IAO_0000114> rdf:type owl:AnnotationProperty .


###  http://purl.obolibrary.org/obo/IAO_0000115
<http://purl.obolibrary.org/obo/IAO_0000115> rdf:type owl:AnnotationProperty .


###  http://purl.obolibrary.org/obo/IAO_0000117
<http://purl.obolibrary.org/obo/IAO_0000117> rdf:type owl:AnnotationProperty .


###  http://purl.obolibrary.org/obo/IAO_0000119
<http://purl.obolibrary.org/obo/IAO_0000119> rdf:type owl:AnnotationProperty .


###  http://purl.org/dc/elements/1.1/date
<http://purl.org/dc/elements/1.1/date> rdf:type owl:AnnotationProperty .


###  http://purl.org/dc/elements/1.1/license
<http://purl.org/dc/elements/1.1/license> rdf:type owl:AnnotationProperty .


###  http://purl.org/dc/terms/license
<http://purl.org/dc/terms/license> rdf:type owl:AnnotationProperty .


###  http://purl.org/dc/terms/rightsHolder
<http://purl.org/dc/terms/rightsHolder> rdf:type owl:AnnotationProperty .


###  http://schema.org/image
<http://schema.org/image> rdf:type owl:AnnotationProperty .


###  http://www.geneontology.org/formats/oboInOwl#hasExactSynonym
<http://www.geneontology.org/formats/oboInOwl#hasExactSynonym> rdf:type owl:AnnotationProperty .


#################################################################
#    Object Properties
#################################################################

###  http://purl.obolibrary.org/obo/RO_0001000
<http://purl.obolibrary.org/obo/RO_0001000> rdf:type owl:ObjectProperty .


#################################################################
#    Classes
#################################################################

###  http://purl.obolibrary.org/obo/FOODON_00002577
<http://purl.obolibrary.org/obo/FOODON_00002577> rdf:type owl:Class ;
                                                 rdfs:label "wine by region"@en .


###  http://purl.obolibrary.org/obo/FOODON_00002583
<http://purl.obolibrary.org/obo/FOODON_00002583> rdf:type owl:Class ;
                                                 rdfs:subClassOf <http://purl.obolibrary.org/obo/FOODON_03412121> ;
                                                 <http://purl.obolibrary.org/obo/IAO_0000114> <http://purl.obolibrary.org/obo/IAO_0000122> ;
                                                 <http://purl.obolibrary.org/obo/IAO_0000115> "The Chardonnay grape plant is the result of a cross between the Pinot noir and Gouais blanc (Heunisch) grape varieties. It produces a green-skinned grape variety used in the production of white wine."@en ;
                                                 <http://purl.obolibrary.org/obo/IAO_0000119> "https://en.wikipedia.org/wiki/Chardonnay" ;
                                                 rdfs:label "Chardonnay grape plant"@en .


###  http://purl.obolibrary.org/obo/FOODON_00002584
<http://purl.obolibrary.org/obo/FOODON_00002584> rdf:type owl:Class ;
                                                 rdfs:subClassOf <http://purl.obolibrary.org/obo/FOODON_03310273> ,
                                                                 [ owl:intersectionOf ( [ rdf:type owl:Restriction ;
                                                                                          owl:onProperty <http://purl.obolibrary.org/obo/RO_0001000> ;
                                                                                          owl:someValuesFrom <http://purl.obolibrary.org/obo/FOODON_00002583>
                                                                                        ]
                                                                                        [ rdf:type owl:Restriction ;
                                                                                          owl:onProperty <http://purl.obolibrary.org/obo/RO_0001000> ;
                                                                                          owl:allValuesFrom <http://purl.obolibrary.org/obo/FOODON_00002583>
                                                                                        ]
                                                                                      ) ;
                                                                   rdf:type owl:Class
                                                                 ] ;
                                                 <http://purl.obolibrary.org/obo/IAO_0000114> <http://purl.obolibrary.org/obo/IAO_0000122> ;
                                                 <http://purl.obolibrary.org/obo/IAO_0000115> "Chardonnay wine is wine produced using only Chardonnay grapes."@en ;
                                                 <http://purl.obolibrary.org/obo/IAO_0000117> "Emma Griffiths" ;
                                                 <http://purl.obolibrary.org/obo/IAO_0000119> "https://en.wikipedia.org/wiki/Chardonnay" ;
                                                 rdfs:label "Chardonnay wine"@en .


###  http://purl.obolibrary.org/obo/FOODON_00002585
<http://purl.obolibrary.org/obo/FOODON_00002585> rdf:type owl:Class ;
                                                 rdfs:subClassOf <http://purl.obolibrary.org/obo/FOODON_03310272> ,
                                                                 [ owl:intersectionOf ( [ rdf:type owl:Restriction ;
                                                                                          owl:onProperty <http://purl.obolibrary.org/obo/RO_0001000> ;
                                                                                          owl:someValuesFrom <http://purl.obolibrary.org/obo/FOODON_00002640>
                                                                                        ]
                                                                                        [ rdf:type owl:Restriction ;
                                                                                          owl:onProperty <http://purl.obolibrary.org/obo/RO_0001000> ;
                                                                                          owl:allValuesFrom <http://purl.obolibrary.org/obo/FOODON_00002640>
                                                                                        ]
                                                                                      ) ;
                                                                   rdf:type owl:Class
                                                                 ] ;
                                                 <http://purl.obolibrary.org/obo/IAO_0000114> <http://purl.obolibrary.org/obo/IAO_0000122> ;
                                                 <http://purl.obolibrary.org/obo/IAO_0000115> "A Cabernet Sauvignon wine is any wine produced using only Cabernet Sauvignon grapes. It often appears with Merlot and Cabernet Franc in blended Bordeaux wines."@en ;
                                                 <http://purl.obolibrary.org/obo/IAO_0000117> "Damion Dooley" ;
                                                 <http://purl.obolibrary.org/obo/IAO_0000119> "https://en.wikipedia.org/wiki/Cabernet_Sauvignon" ;
                                                 rdfs:label "Cabernet Sauvignon wine"@en .


###  http://purl.obolibrary.org/obo/FOODON_00002586
<http://purl.obolibrary.org/obo/FOODON_00002586> rdf:type owl:Class ;
                                                 rdfs:subClassOf <http://purl.obolibrary.org/obo/FOODON_03310273> ,
                                                                 [ owl:intersectionOf ( [ rdf:type owl:Restriction ;
                                                                                          owl:onProperty <http://purl.obolibrary.org/obo/RO_0001000> ;
                                                                                          owl:someValuesFrom <http://purl.obolibrary.org/obo/FOODON_00002587>
                                                                                        ]
                                                                                        [ rdf:type owl:Restriction ;
                                                                                          owl:onProperty <http://purl.obolibrary.org/obo/RO_0001000> ;
                                                                                          owl:allValuesFrom <http://purl.obolibrary.org/obo/FOODON_00002587>
                                                                                        ]
                                                                                      ) ;
                                                                   rdf:type owl:Class
                                                                 ] ;
                                                 <http://purl.obolibrary.org/obo/IAO_0000114> <http://purl.obolibrary.org/obo/IAO_0000122> ;
                                                 <http://purl.obolibrary.org/obo/IAO_0000115> "A Chenin blanc wine is any wine produced using only Chenin blanc grapes."@en ;
                                                 <http://purl.obolibrary.org/obo/IAO_0000117> "Lauren Tindale" ;
                                                 rdfs:label "Chenin blanc wine"@en .


###  http://purl.obolibrary.org/obo/FOODON_00002587
<http://purl.obolibrary.org/obo/FOODON_00002587> rdf:type owl:Class ;
                                                 rdfs:subClassOf <http://purl.obolibrary.org/obo/FOODON_03412121> ;
                                                 <http://purl.obolibrary.org/obo/IAO_0000114> <http://purl.obolibrary.org/obo/IAO_0000122> ;
                                                 <http://purl.obolibrary.org/obo/IAO_0000115> "Chenin blanc grapes are a White wine grape variety from the Loire Valley of France. Its high acidity means it can be used to make everything from sparkling wines to well-balanced dessert wines, although it can produce very bland, neutral wines if the vine's natural vigor is not controlled."@en ;
                                                 <http://purl.obolibrary.org/obo/IAO_0000117> "Lauren Tindale" ;
                                                 <http://purl.obolibrary.org/obo/IAO_0000119> "https://en.wikipedia.org/wiki/Chenin_blanc" ;
                                                 <http://www.geneontology.org/formats/oboInOwl#hasExactSynonym> "Pineau de la Loire"@fr ;
                                                 rdfs:label "Chenin blanc grape plant"@en .


###  http://purl.obolibrary.org/obo/FOODON_00002588
<http://purl.obolibrary.org/obo/FOODON_00002588> rdf:type owl:Class ;
                                                 rdfs:subClassOf <http://purl.obolibrary.org/obo/FOODON_03310272> ,
                                                                 [ owl:intersectionOf ( [ rdf:type owl:Restriction ;
                                                                                          owl:onProperty <http://purl.obolibrary.org/obo/RO_0001000> ;
                                                                                          owl:someValuesFrom <http://purl.obolibrary.org/obo/FOODON_00002589>
                                                                                        ]
                                                                                        [ rdf:type owl:Restriction ;
                                                                                          owl:onProperty <http://purl.obolibrary.org/obo/RO_0001000> ;
                                                                                          owl:allValuesFrom <http://purl.obolibrary.org/obo/FOODON_00002589>
                                                                                        ]
                                                                                      ) ;
                                                                   rdf:type owl:Class
                                                                 ] ;
                                                 <http://purl.obolibrary.org/obo/IAO_0000114> <http://purl.obolibrary.org/obo/IAO_0000122> ;
                                                 <http://purl.obolibrary.org/obo/IAO_0000115> "A Malbec wine is any wine produced using only Malbec grapes."@en ;
                                                 <http://purl.obolibrary.org/obo/IAO_0000117> "Lauren Tindale" ;
                                                 rdfs:label "Malbec wine"@en .


###  http://purl.obolibrary.org/obo/FOODON_00002589
<http://purl.obolibrary.org/obo/FOODON_00002589> rdf:type owl:Class ;
                                                 rdfs:subClassOf <http://purl.obolibrary.org/obo/FOODON_03412121> ;
                                                 <http://purl.obolibrary.org/obo/IAO_0000114> <http://purl.obolibrary.org/obo/IAO_0000122> ;
                                                 <http://purl.obolibrary.org/obo/IAO_0000115> "Malbec grapes are a purple grape variety used in making red wine. The grapes tend to have an inky dark color and robust tannins, and are known as one of the six grapes allowed in the blend of red Bordeaux wine. The French plantations of Malbec are now found primarily in Cahors in South West France. It is increasingly celebrated as an Argentine varietal wine and is being grown around the world."@en ;
                                                 <http://purl.obolibrary.org/obo/IAO_0000117> "Lauren Tindale" ;
                                                 <http://purl.obolibrary.org/obo/IAO_0000119> "https://en.wikipedia.org/wiki/Malbec" ;
                                                 rdfs:label "Malbec grape plant"@en .


###  http://purl.obolibrary.org/obo/FOODON_00002590
<http://purl.obolibrary.org/obo/FOODON_00002590> rdf:type owl:Class ;
                                                 rdfs:subClassOf <http://purl.obolibrary.org/obo/FOODON_03310272> ,
                                                                 [ owl:intersectionOf ( [ rdf:type owl:Restriction ;
                                                                                          owl:onProperty <http://purl.obolibrary.org/obo/RO_0001000> ;
                                                                                          owl:someValuesFrom <http://purl.obolibrary.org/obo/FOODON_00002591>
                                                                                        ]
                                                                                        [ rdf:type owl:Restriction ;
                                                                                          owl:onProperty <http://purl.obolibrary.org/obo/RO_0001000> ;
                                                                                          owl:allValuesFrom <http://purl.obolibrary.org/obo/FOODON_00002591>
                                                                                        ]
                                                                                      ) ;
                                                                   rdf:type owl:Class
                                                                 ] ;
                                                 <http://purl.obolibrary.org/obo/IAO_0000114> <http://purl.obolibrary.org/obo/IAO_0000122> ;
                                                 <http://purl.obolibrary.org/obo/IAO_0000115> "A Merlot wine is any wine produced using only Merlot grapes."@en ;
                                                 <http://purl.obolibrary.org/obo/IAO_0000117> "Lauren Tindale" ;
                                                 rdfs:label "Merlot wine"@en .


###  http://purl.obolibrary.org/obo/FOODON_00002591
<http://purl.obolibrary.org/obo/FOODON_00002591> rdf:type owl:Class ;
                                                 rdfs:subClassOf <http://purl.obolibrary.org/obo/FOODON_03412121> ;
                                                 <http://purl.obolibrary.org/obo/IAO_0000114> <http://purl.obolibrary.org/obo/IAO_0000122> ;
                                                 <http://purl.obolibrary.org/obo/IAO_0000115> "Merlot is a dark blue-colored wine grape variety, that is used as both a blending grape and for varietal wines."@en ;
                                                 <http://purl.obolibrary.org/obo/IAO_0000117> "Lauren Tindale" ;
                                                 <http://purl.obolibrary.org/obo/IAO_0000119> "https://en.wikipedia.org/wiki/Merlot" ;
                                                 <http://schema.org/image> <https://upload.wikimedia.org/wikipedia/commons/thumb/e/ee/Merlot_Grape.jpg/320px-Merlot_Grape.jpg> ;
                                                 rdfs:label "Merlot grape plant"@en .


###  http://purl.obolibrary.org/obo/FOODON_00002592
<http://purl.obolibrary.org/obo/FOODON_00002592> rdf:type owl:Class ;
                                                 rdfs:subClassOf <http://purl.obolibrary.org/obo/FOODON_03310273> ,
                                                                 [ owl:intersectionOf ( [ rdf:type owl:Restriction ;
                                                                                          owl:onProperty <http://purl.obolibrary.org/obo/RO_0001000> ;
                                                                                          owl:someValuesFrom <http://purl.obolibrary.org/obo/FOODON_00002593>
                                                                                        ]
                                                                                        [ rdf:type owl:Restriction ;
                                                                                          owl:onProperty <http://purl.obolibrary.org/obo/RO_0001000> ;
                                                                                          owl:allValuesFrom <http://purl.obolibrary.org/obo/FOODON_00002593>
                                                                                        ]
                                                                                      ) ;
                                                                   rdf:type owl:Class
                                                                 ] ;
                                                 <http://purl.obolibrary.org/obo/IAO_0000114> <http://purl.obolibrary.org/obo/IAO_0000122> ;
                                                 <http://purl.obolibrary.org/obo/IAO_0000115> "A pinot blanc wine is any wine produced using only Pinco blanc grapes."@en ;
                                                 <http://purl.obolibrary.org/obo/IAO_0000117> "Lauren Tindale" ;
                                                 rdfs:label "Pinot blanc wine"@en .


###  http://purl.obolibrary.org/obo/FOODON_00002593
<http://purl.obolibrary.org/obo/FOODON_00002593> rdf:type owl:Class ;
                                                 rdfs:subClassOf <http://purl.obolibrary.org/obo/FOODON_03412121> ;
                                                 <http://purl.obolibrary.org/obo/IAO_0000114> <http://purl.obolibrary.org/obo/IAO_0000122> ;
                                                 <http://purl.obolibrary.org/obo/IAO_0000115> "Pinot blanc is a white wine grape. It is a point genetic mutation of Pinot noir."@en ;
                                                 <http://purl.obolibrary.org/obo/IAO_0000117> "Lauren Tindale" ;
                                                 <http://purl.obolibrary.org/obo/IAO_0000119> "https://en.wikipedia.org/wiki/Pinot_blanc" ;
                                                 <http://schema.org/image> <https://upload.wikimedia.org/wikipedia/commons/thumb/b/b3/Pinot-blanc.jpg/440px-Pinot-blanc.jpg> ;
                                                 rdfs:label "Pinot blanc grape plant"@en .


###  http://purl.obolibrary.org/obo/FOODON_00002594
<http://purl.obolibrary.org/obo/FOODON_00002594> rdf:type owl:Class ;
                                                 rdfs:subClassOf <http://purl.obolibrary.org/obo/FOODON_03310273> ,
                                                                 [ owl:intersectionOf ( [ rdf:type owl:Restriction ;
                                                                                          owl:onProperty <http://purl.obolibrary.org/obo/RO_0001000> ;
                                                                                          owl:someValuesFrom <http://purl.obolibrary.org/obo/FOODON_00002595>
                                                                                        ]
                                                                                        [ rdf:type owl:Restriction ;
                                                                                          owl:onProperty <http://purl.obolibrary.org/obo/RO_0001000> ;
                                                                                          owl:allValuesFrom <http://purl.obolibrary.org/obo/FOODON_00002595>
                                                                                        ]
                                                                                      ) ;
                                                                   rdf:type owl:Class
                                                                 ] ;
                                                 <http://purl.obolibrary.org/obo/IAO_0000114> <http://purl.obolibrary.org/obo/IAO_0000122> ;
                                                 <http://purl.obolibrary.org/obo/IAO_0000115> "Pinot gris is a white wine varietal produced only from Pinot gris grapes.  The Italian synonym, Pinot Grigio, has become strongly associated with lighter wines produced in great quantities, particularly in northern Italy."@en ;
                                                 <http://purl.obolibrary.org/obo/IAO_0000117> "Ginny Pichler" ;
                                                 <http://purl.obolibrary.org/obo/IAO_0000119> "https://www.wine-searcher.com/grape-381-pinot-grigio" ;
                                                 <http://schema.org/image> <https://upload.wikimedia.org/wikipedia/commons/thumb/5/59/Alto_adige_Pinot_grigio.jpg/179px-Alto_adige_Pinot_grigio.jpg> ;
                                                 <http://www.geneontology.org/formats/oboInOwl#hasExactSynonym> "Grauburgunder"@ge ,
                                                                                                                "Pinot Grigio"@it ;
                                                 rdfs:label "Pinot gris wine"@en .


###  http://purl.obolibrary.org/obo/FOODON_00002595
<http://purl.obolibrary.org/obo/FOODON_00002595> rdf:type owl:Class ;
                                                 rdfs:subClassOf <http://purl.obolibrary.org/obo/FOODON_03412121> ;
                                                 <http://purl.obolibrary.org/obo/IAO_0000114> <http://purl.obolibrary.org/obo/IAO_0000122> ;
                                                 <http://purl.obolibrary.org/obo/IAO_0000115> "Pinot gris is a white wine grape variety (mutation) of the Pinot family which shares its genetic fingerprint with Pinot Noir, Pinot Blanc et al. . Pinot gris is grown around the globe with the \"spicy\" full-bodied Alsatian and lighter-bodied, more acidic Italian styles being most widely recognized."@en ;
                                                 <http://purl.obolibrary.org/obo/IAO_0000117> "Ginny Pichler" ;
                                                 <http://purl.obolibrary.org/obo/IAO_0000119> "https://en.wikipedia.org/wiki/Pinot_gris" ;
                                                 <http://schema.org/image> <https://commons.wikimedia.org/wiki/File:Pinot_Gris_close.JPG> ;
                                                 <http://www.geneontology.org/formats/oboInOwl#hasExactSynonym> "Grauburgunder"@ge ,
                                                                                                                "Pinot Grigio grape"@it ;
                                                 rdfs:label "Pinot gris grape plant"@en .


###  http://purl.obolibrary.org/obo/FOODON_00002596
<http://purl.obolibrary.org/obo/FOODON_00002596> rdf:type owl:Class ;
                                                 rdfs:subClassOf <http://purl.obolibrary.org/obo/FOODON_03310272> ,
                                                                 [ owl:intersectionOf ( [ rdf:type owl:Restriction ;
                                                                                          owl:onProperty <http://purl.obolibrary.org/obo/RO_0001000> ;
                                                                                          owl:someValuesFrom <http://purl.obolibrary.org/obo/FOODON_00002597>
                                                                                        ]
                                                                                        [ rdf:type owl:Restriction ;
                                                                                          owl:onProperty <http://purl.obolibrary.org/obo/RO_0001000> ;
                                                                                          owl:allValuesFrom <http://purl.obolibrary.org/obo/FOODON_00002597>
                                                                                        ]
                                                                                      ) ;
                                                                   rdf:type owl:Class
                                                                 ] ;
                                                 <http://purl.obolibrary.org/obo/IAO_0000114> <http://purl.obolibrary.org/obo/IAO_0000122> ;
                                                 <http://purl.obolibrary.org/obo/IAO_0000115> "Pinot noir wine is a red wine varietal made only from Pinot noir grapes.  The thin skins and low levels of phenolic compounds lends pinot to producing mostly lightly colored, medium-bodied and low-tannin wines that can often go through phases of uneven and unpredictable aging."@en ;
                                                 <http://purl.obolibrary.org/obo/IAO_0000117> "Shannon Russell" ;
                                                 <http://purl.obolibrary.org/obo/IAO_0000119> "https://en.wikipedia.org/wiki/Pinot_noir" ;
                                                 <http://www.geneontology.org/formats/oboInOwl#hasExactSynonym> "Blauburgunder"@ge ,
                                                                                                                "Pinot Nero"@fr ,
                                                                                                                "Rulandské modré"@fr ,
                                                                                                                "Spätburgunder"@ge ;
                                                 rdfs:label "Pinot noir wine"@en .


###  http://purl.obolibrary.org/obo/FOODON_00002597
<http://purl.obolibrary.org/obo/FOODON_00002597> rdf:type owl:Class ;
                                                 rdfs:subClassOf <http://purl.obolibrary.org/obo/FOODON_03412121> ;
                                                 <http://purl.obolibrary.org/obo/IAO_0000114> <http://purl.obolibrary.org/obo/IAO_0000122> ;
                                                 <http://purl.obolibrary.org/obo/IAO_0000115> "Pinot noir grape is a red wine grape variety. The name is derived from the French words for pine and black. The word pine alludes to the grape variety having tightly clustered, pine cone-shaped bunches of fruit. Pinot noir grapes are grown around the world, mostly in the cooler climates, and the grape is chiefly associated with the Burgundy region of France."@en ;
                                                 <http://purl.obolibrary.org/obo/IAO_0000117> "Shannon Russell" ;
                                                 <http://purl.obolibrary.org/obo/IAO_0000119> "https://en.wikipedia.org/wiki/Pinot_noir" ;
                                                 <http://schema.org/image> <https://en.wikipedia.org/wiki/Pinot_noir#/media/File:Grape_near_Sancerre.jpg> ;
                                                 rdfs:label "Pinot noir grape plant"@en .


###  http://purl.obolibrary.org/obo/FOODON_00002598
<http://purl.obolibrary.org/obo/FOODON_00002598> rdf:type owl:Class ;
                                                 rdfs:subClassOf <http://purl.obolibrary.org/obo/FOODON_03310272> ,
                                                                 [ owl:intersectionOf ( [ rdf:type owl:Restriction ;
                                                                                          owl:onProperty <http://purl.obolibrary.org/obo/RO_0001000> ;
                                                                                          owl:someValuesFrom <http://purl.obolibrary.org/obo/FOODON_00002599>
                                                                                        ]
                                                                                        [ rdf:type owl:Restriction ;
                                                                                          owl:onProperty <http://purl.obolibrary.org/obo/RO_0001000> ;
                                                                                          owl:allValuesFrom <http://purl.obolibrary.org/obo/FOODON_00002599>
                                                                                        ]
                                                                                      ) ;
                                                                   rdf:type owl:Class
                                                                 ] ;
                                                 <http://purl.obolibrary.org/obo/IAO_0000114> <http://purl.obolibrary.org/obo/IAO_0000122> ;
                                                 <http://purl.obolibrary.org/obo/IAO_0000115> "Pinotage wine is a red wine varietal produced only from Pinotage grapes. This type of wine can range from a fairly cheap, light-bodied red wine with some funky aromas (including extremes such as acetone, paint, rubber, and at times banana) all the way to full-bodied red wines with balance, elegance, fully developed black fruit flavors, and an enduring, sweet, smokey finish."@en ;
                                                 <http://purl.obolibrary.org/obo/IAO_0000117> "Ginny Pichler" ;
                                                 <http://purl.obolibrary.org/obo/IAO_0000119> "https://www.thespruceeats.com/what-is-pinotage-wine-3511226" ;
                                                 <http://schema.org/image> <https://upload.wikimedia.org/wikipedia/commons/thumb/e/e4/Stellenbosch_Pinotage.jpg/179px-Stellenbosch_Pinotage.jpg> ;
                                                 rdfs:label "Pinotage wine"@en .


###  http://purl.obolibrary.org/obo/FOODON_00002599
<http://purl.obolibrary.org/obo/FOODON_00002599> rdf:type owl:Class ;
                                                 rdfs:subClassOf <http://purl.obolibrary.org/obo/FOODON_03412121> ;
                                                 <http://purl.obolibrary.org/obo/IAO_0000114> <http://purl.obolibrary.org/obo/IAO_0000122> ;
                                                 <http://purl.obolibrary.org/obo/IAO_0000115> "Pinotage is a red wine grape that is South Africa's signature variety. It was bred there in 1925 as a crossbetween Pinot noir and Cinsaut. The grape is a viticultural intraspecific cross of two varieties of Vitis vinifera, not an interspecific hybrid."@en ;
                                                 <http://purl.obolibrary.org/obo/IAO_0000117> "Ginny Pichler" ;
                                                 <http://purl.obolibrary.org/obo/IAO_0000119> "https://en.wikipedia.org/wiki/Pinotage" ;
                                                 <http://schema.org/image> <https://i2.wp.com/www.winetwofive.com/wp-content/uploads/2018/06/CEP-TIBOUREN.jpg?resize=128%2C128> ;
                                                 rdfs:label "Pinotage grape plant"@en .


###  http://purl.obolibrary.org/obo/FOODON_00002600
<http://purl.obolibrary.org/obo/FOODON_00002600> rdf:type owl:Class ;
                                                 rdfs:subClassOf <http://purl.obolibrary.org/obo/FOODON_03301014> ;
                                                 <http://purl.obolibrary.org/obo/IAO_0000114> <http://purl.obolibrary.org/obo/IAO_0000122> ;
                                                 <http://purl.obolibrary.org/obo/IAO_0000115> "Reserve wine is wine of a higher quality than usual, or a wine that has been aged before being sold, or both. Traditionally, winemakers would reserve some of their best wine rather than sell it immediately, coining the term."@en ;
                                                 <http://purl.obolibrary.org/obo/IAO_0000117> "Damion Dooley" ;
                                                 <http://purl.obolibrary.org/obo/IAO_0000119> "https://en.wikipedia.org/wiki/Reserve_wine" ;
                                                 rdfs:label "Reserve wine"@en .


###  http://purl.obolibrary.org/obo/FOODON_00002601
<http://purl.obolibrary.org/obo/FOODON_00002601> rdf:type owl:Class ;
                                                 rdfs:subClassOf <http://purl.obolibrary.org/obo/FOODON_03310273> ,
                                                                 [ owl:intersectionOf ( [ rdf:type owl:Restriction ;
                                                                                          owl:onProperty <http://purl.obolibrary.org/obo/RO_0001000> ;
                                                                                          owl:someValuesFrom <http://purl.obolibrary.org/obo/FOODON_00002602>
                                                                                        ]
                                                                                        [ rdf:type owl:Restriction ;
                                                                                          owl:onProperty <http://purl.obolibrary.org/obo/RO_0001000> ;
                                                                                          owl:allValuesFrom <http://purl.obolibrary.org/obo/FOODON_00002602>
                                                                                        ]
                                                                                      ) ;
                                                                   rdf:type owl:Class
                                                                 ] ;
                                                 <http://purl.obolibrary.org/obo/IAO_0000114> <http://purl.obolibrary.org/obo/IAO_0000122> ;
                                                 <http://purl.obolibrary.org/obo/IAO_0000115> "Riesling wine is a white wine varietal produced only from Riesling grapes, and offered as dry, semi-sweet, sweet, and sparkling white wines. Riesling wines are usually varietally pure and are seldom oaked."@en ;
                                                 <http://purl.obolibrary.org/obo/IAO_0000117> "Ginny Pichler" ;
                                                 <http://purl.obolibrary.org/obo/IAO_0000119> "https://en.wikipedia.org/wiki/Riesling" ;
                                                 <http://schema.org/image> <https://upload.wikimedia.org/wikipedia/commons/thumb/9/96/Alsatian_Riesling_.jpg/179px-Alsatian_Riesling_.jpg> ;
                                                 rdfs:label "Riesling wine"@en .


###  http://purl.obolibrary.org/obo/FOODON_00002602
<http://purl.obolibrary.org/obo/FOODON_00002602> rdf:type owl:Class ;
                                                 rdfs:subClassOf <http://purl.obolibrary.org/obo/FOODON_03412121> ;
                                                 <http://purl.obolibrary.org/obo/IAO_0000114> <http://purl.obolibrary.org/obo/IAO_0000122> ;
                                                 <http://purl.obolibrary.org/obo/IAO_0000115> "Riesling grape is an aromatic white grape variety displaying flowery, almost perfumed, aromas as well as high acidity."@en ;
                                                 <http://purl.obolibrary.org/obo/IAO_0000117> "Ginny Pichler" ;
                                                 <http://purl.obolibrary.org/obo/IAO_0000119> "https://en.wikipedia.org/wiki/Riesling" ;
                                                 <http://schema.org/image> <https://upload.wikimedia.org/wikipedia/commons/thumb/7/76/Riesling_grapes_leaves.jpg/320px-Riesling_grapes_leaves.jpg> ;
                                                 rdfs:label "Riesling grape plant"@en .


###  http://purl.obolibrary.org/obo/FOODON_00002603
<http://purl.obolibrary.org/obo/FOODON_00002603> rdf:type owl:Class ;
                                                 rdfs:subClassOf <http://purl.obolibrary.org/obo/FOODON_03310272> ,
                                                                 [ owl:intersectionOf ( [ rdf:type owl:Restriction ;
                                                                                          owl:onProperty <http://purl.obolibrary.org/obo/RO_0001000> ;
                                                                                          owl:someValuesFrom <http://purl.obolibrary.org/obo/FOODON_00002604>
                                                                                        ]
                                                                                        [ rdf:type owl:Restriction ;
                                                                                          owl:onProperty <http://purl.obolibrary.org/obo/RO_0001000> ;
                                                                                          owl:allValuesFrom <http://purl.obolibrary.org/obo/FOODON_00002604>
                                                                                        ]
                                                                                      ) ;
                                                                   rdf:type owl:Class
                                                                 ] ;
                                                 <http://purl.obolibrary.org/obo/IAO_0000114> <http://purl.obolibrary.org/obo/IAO_0000122> ;
                                                 <http://purl.obolibrary.org/obo/IAO_0000115> "Sangiovese wine is a red wine varietal produced only from Sangiovese grapes. It is prized for its high acid, firm tannins and balanced nature. Savory flavors of dark cherries and black stonefruit are characteristic, and may be backed by secondary notes of tomato leaf and dried herbs."@en ;
                                                 <http://purl.obolibrary.org/obo/IAO_0000117> "Ginny Pichler" ;
                                                 <http://purl.obolibrary.org/obo/IAO_0000119> "https://www.wine-searcher.com/grape-432-sangiovese" ;
                                                 <http://schema.org/image> <https://upload.wikimedia.org/wikipedia/commons/thumb/2/2e/Sangiovese_wine.jpg/180px-Sangiovese_wine.jpg> ;
                                                 rdfs:label "Sangiovese wine"@en .


###  http://purl.obolibrary.org/obo/FOODON_00002604
<http://purl.obolibrary.org/obo/FOODON_00002604> rdf:type owl:Class ;
                                                 rdfs:subClassOf <http://purl.obolibrary.org/obo/FOODON_03412121> ;
                                                 <http://purl.obolibrary.org/obo/IAO_0000114> <http://purl.obolibrary.org/obo/IAO_0000122> ;
                                                 <http://purl.obolibrary.org/obo/IAO_0000115> "Sangiovese is a red Italian wine grape variety that derives its name from the Latin sanguis Jovis, \"the blood of Jupiter\"."@en ;
                                                 <http://purl.obolibrary.org/obo/IAO_0000117> "Ginny Pichler" ;
                                                 <http://purl.obolibrary.org/obo/IAO_0000119> "https://en.wikipedia.org/wiki/Sangiovese" ;
                                                 <http://schema.org/image> <https://upload.wikimedia.org/wikipedia/commons/thumb/3/37/Sangiovese_close_up_crop.jpg/277px-Sangiovese_close_up_crop.jpg> ;
                                                 rdfs:label "Sangiovese grape plant"@en .


###  http://purl.obolibrary.org/obo/FOODON_00002605
<http://purl.obolibrary.org/obo/FOODON_00002605> rdf:type owl:Class ;
                                                 rdfs:subClassOf <http://purl.obolibrary.org/obo/FOODON_03310273> ,
                                                                 [ owl:intersectionOf ( [ rdf:type owl:Restriction ;
                                                                                          owl:onProperty <http://purl.obolibrary.org/obo/RO_0001000> ;
                                                                                          owl:someValuesFrom <http://purl.obolibrary.org/obo/FOODON_00002606>
                                                                                        ]
                                                                                        [ rdf:type owl:Restriction ;
                                                                                          owl:onProperty <http://purl.obolibrary.org/obo/RO_0001000> ;
                                                                                          owl:allValuesFrom <http://purl.obolibrary.org/obo/FOODON_00002606>
                                                                                        ]
                                                                                      ) ;
                                                                   rdf:type owl:Class
                                                                 ] ;
                                                 <http://purl.obolibrary.org/obo/IAO_0000114> <http://purl.obolibrary.org/obo/IAO_0000122> ;
                                                 <http://purl.obolibrary.org/obo/IAO_0000115> "Sauvignon blanc wine is a white wine varietal produced only from Sauvignon blanc grapes.  Its primary fruit flavors are lime, green apple, passion fruit and white peach. Depending on how ripe the grapes are when the wine is made, the flavor will range from zesty lime to flowery peach."@en ;
                                                 <http://purl.obolibrary.org/obo/IAO_0000117> "Shannon Russell" ;
                                                 <http://purl.obolibrary.org/obo/IAO_0000119> "https://winefolly.com/review/sauvignon-blanc-wine-taste-food-pairing/" ;
                                                 <http://www.geneontology.org/formats/oboInOwl#hasExactSynonym> "Blanc fume"@fr ,
                                                                                                                "Fume blanc"@fr ,
                                                                                                                "Muskat-Silvaner"@en ,
                                                                                                                "Sauvignon jaune"@fr ;
                                                 rdfs:label "Sauvignon blanc wine"@en .


###  http://purl.obolibrary.org/obo/FOODON_00002606
<http://purl.obolibrary.org/obo/FOODON_00002606> rdf:type owl:Class ;
                                                 rdfs:subClassOf <http://purl.obolibrary.org/obo/FOODON_03412121> ;
                                                 <http://purl.obolibrary.org/obo/IAO_0000114> <http://purl.obolibrary.org/obo/IAO_0000122> ;
                                                 <http://purl.obolibrary.org/obo/IAO_0000115> "Sauvignon blanc is a green-skinned grape variety that originates from the Bordeaux region of France. The grape most likely gets its name from the French words sauvage (\"wild\") and blanc (\"white\") due to its early origins as an indigenous grape in South West France."@en ;
                                                 <http://purl.obolibrary.org/obo/IAO_0000117> "Shannon Russell" ;
                                                 <http://purl.obolibrary.org/obo/IAO_0000119> "https://en.wikipedia.org/wiki/Sauvignon_blanc" ;
                                                 <http://schema.org/image> <https://upload.wikimedia.org/wikipedia/commons/thumb/5/50/Sauvignon_blanc_grapes.jpg/360px-Sauvignon_blanc_grapes.jpg> ;
                                                 rdfs:label "Sauvignon blanc grape plant"@en .


###  http://purl.obolibrary.org/obo/FOODON_00002607
<http://purl.obolibrary.org/obo/FOODON_00002607> rdf:type owl:Class ;
                                                 rdfs:subClassOf <http://purl.obolibrary.org/obo/FOODON_03310273> ,
                                                                 [ owl:intersectionOf ( [ rdf:type owl:Restriction ;
                                                                                          owl:onProperty <http://purl.obolibrary.org/obo/RO_0001000> ;
                                                                                          owl:someValuesFrom <http://purl.obolibrary.org/obo/FOODON_00002608>
                                                                                        ]
                                                                                        [ rdf:type owl:Restriction ;
                                                                                          owl:onProperty <http://purl.obolibrary.org/obo/RO_0001000> ;
                                                                                          owl:allValuesFrom <http://purl.obolibrary.org/obo/FOODON_00002608>
                                                                                        ]
                                                                                      ) ;
                                                                   rdf:type owl:Class
                                                                 ] ;
                                                 <http://purl.obolibrary.org/obo/IAO_0000114> <http://purl.obolibrary.org/obo/IAO_0000122> ;
                                                 <http://purl.obolibrary.org/obo/IAO_0000115> "Semillon wine is a white wine varietal produced only from Semillon grapes.  The primary fruit flavors in Semillon wine are lemon, apple, pear and green papaya. Semillon is France’s 3rd most planted white wine variety behind Sauvignon Blanc and Chardonnay."@en ;
                                                 <http://purl.obolibrary.org/obo/IAO_0000117> "Ginny Pichler" ;
                                                 <http://purl.obolibrary.org/obo/IAO_0000119> "https://winefolly.com/review/have-you-heard-of-semillon-the-3rd-most-important-french-white-wine/" ;
                                                 <http://schema.org/image> <https://upload.wikimedia.org/wikipedia/commons/thumb/1/1d/Late_harvest_Semillon.jpg/179px-Late_harvest_Semillon.jpg> ;
                                                 <http://www.geneontology.org/formats/oboInOwl#hasExactSynonym> "Sémillon wine"@fr ;
                                                 rdfs:label "Semillon wine"@en .


###  http://purl.obolibrary.org/obo/FOODON_00002608
<http://purl.obolibrary.org/obo/FOODON_00002608> rdf:type owl:Class ;
                                                 rdfs:subClassOf <http://purl.obolibrary.org/obo/FOODON_03412121> ;
                                                 <http://purl.obolibrary.org/obo/IAO_0000114> <http://purl.obolibrary.org/obo/IAO_0000122> ;
                                                 <http://purl.obolibrary.org/obo/IAO_0000115> "Semillon is a golden-skinned grape used to make dry and sweet white wines, mostly in France and Australia."@en ;
                                                 <http://purl.obolibrary.org/obo/IAO_0000117> "Ginny Pichler" ;
                                                 <http://purl.obolibrary.org/obo/IAO_0000119> "https://en.wikipedia.org/wiki/S%C3%A9millon" ;
                                                 <http://schema.org/image> <https://upload.wikimedia.org/wikipedia/commons/thumb/2/27/Semillon_starting_to_get_noble_rot_at_Ch%C3%A2teau_Doisy-V%C3%A9drines%2C_Barsac%2C_Sauternes.jpg/160px-Semillon_starting_to_get_noble_rot_at_Ch%C3%A2teau_Doisy-V%C3%A9drines%2C_Barsac%2C_Sauternes.jpg> ;
                                                 <http://www.geneontology.org/formats/oboInOwl#hasExactSynonym> "Sémillon grape"@fr ;
                                                 rdfs:label "Semillon grape plant"@en .


###  http://purl.obolibrary.org/obo/FOODON_00002609
<http://purl.obolibrary.org/obo/FOODON_00002609> rdf:type owl:Class ;
                                                 rdfs:subClassOf <http://purl.obolibrary.org/obo/FOODON_03310273> ,
                                                                 [ owl:intersectionOf ( [ rdf:type owl:Restriction ;
                                                                                          owl:onProperty <http://purl.obolibrary.org/obo/RO_0001000> ;
                                                                                          owl:someValuesFrom <http://purl.obolibrary.org/obo/FOODON_00002610>
                                                                                        ]
                                                                                        [ rdf:type owl:Restriction ;
                                                                                          owl:onProperty <http://purl.obolibrary.org/obo/RO_0001000> ;
                                                                                          owl:allValuesFrom <http://purl.obolibrary.org/obo/FOODON_00002610>
                                                                                        ]
                                                                                      ) ;
                                                                   rdf:type owl:Class
                                                                 ] ;
                                                 <http://purl.obolibrary.org/obo/IAO_0000114> <http://purl.obolibrary.org/obo/IAO_0000122> ;
                                                 <http://purl.obolibrary.org/obo/IAO_0000115> "Glera wine is a white wine varietal produced only from Glera grapes."@en ;
                                                 <http://purl.obolibrary.org/obo/IAO_0000117> "Ginny Pichler" ;
                                                 <http://www.geneontology.org/formats/oboInOwl#hasExactSynonym> "Prosecco wine"@en ;
                                                 rdfs:label "Glera wine"@en .


###  http://purl.obolibrary.org/obo/FOODON_00002610
<http://purl.obolibrary.org/obo/FOODON_00002610> rdf:type owl:Class ;
                                                 rdfs:subClassOf <http://purl.obolibrary.org/obo/FOODON_03412121> ;
                                                 <http://purl.obolibrary.org/obo/IAO_0000114> <http://purl.obolibrary.org/obo/IAO_0000122> ;
                                                 <http://purl.obolibrary.org/obo/IAO_0000115> "Glera is a white variety of grape of Slovenian origin, which was brought to the village of Prosecco from Slovenia's Karst region. Glera was, until 2009, mostly referred to as Prosecco. It is mainly cultivated for use in sparkling Italian wine styles."@en ;
                                                 <http://purl.obolibrary.org/obo/IAO_0000117> "Ginny Pichler" ;
                                                 <http://purl.obolibrary.org/obo/IAO_0000119> "https://en.wikipedia.org/wiki/Glera_(grape)" ;
                                                 <http://schema.org/image> <https://cdn1.wine-searcher.net/images/grape/glera-(prosecco)-392-1-1.jpg> ;
                                                 <http://www.geneontology.org/formats/oboInOwl#hasExactSynonym> "Prosecco grape"@en ;
                                                 rdfs:label "Glera grape plant"@en .


###  http://purl.obolibrary.org/obo/FOODON_00002611
<http://purl.obolibrary.org/obo/FOODON_00002611> rdf:type owl:Class ;
                                                 rdfs:subClassOf <http://purl.obolibrary.org/obo/FOODON_03310273> ,
                                                                 [ owl:intersectionOf ( [ rdf:type owl:Restriction ;
                                                                                          owl:onProperty <http://purl.obolibrary.org/obo/RO_0001000> ;
                                                                                          owl:someValuesFrom <http://purl.obolibrary.org/obo/FOODON_00002610>
                                                                                        ]
                                                                                        [ rdf:type owl:Restriction ;
                                                                                          owl:onProperty <http://purl.obolibrary.org/obo/RO_0001000> ;
                                                                                          owl:allValuesFrom <http://purl.obolibrary.org/obo/FOODON_00002610>
                                                                                        ]
                                                                                      ) ;
                                                                   rdf:type owl:Class
                                                                 ] ;
                                                 <http://purl.obolibrary.org/obo/IAO_0000114> <http://purl.obolibrary.org/obo/IAO_0000122> ;
                                                 <http://purl.obolibrary.org/obo/IAO_0000115> "Prosecco is an Italian white wine varietal produced primarily from Glera grapes, but other grape varieties may be included. Prosecco controlled designation of origin can be spumante (\"sparkling wine\"), frizzante (\"semi-sparkling wine\"), or tranquillo (\"still wine\")."@en ;
                                                 <http://purl.obolibrary.org/obo/IAO_0000117> "Ginny Pichler" ;
                                                 <http://purl.obolibrary.org/obo/IAO_0000119> "https://en.wikipedia.org/wiki/Prosecco" ;
                                                 <http://schema.org/image> <https://upload.wikimedia.org/wikipedia/commons/thumb/c/ce/Prosecco_di_Conegliano_bottle_and_glass.jpg/151px-Prosecco_di_Conegliano_bottle_and_glass.jpg> ;
                                                 <http://www.geneontology.org/formats/oboInOwl#hasExactSynonym> "frizzante"@it ,
                                                                                                                "spumante"@it ,
                                                                                                                "tranquillo"@it ;
                                                 rdfs:label "Prosecco wine"@en .


###  http://purl.obolibrary.org/obo/FOODON_00002612
<http://purl.obolibrary.org/obo/FOODON_00002612> rdf:type owl:Class ;
                                                 rdfs:subClassOf <http://purl.obolibrary.org/obo/FOODON_03310272> ,
                                                                 [ owl:intersectionOf ( [ rdf:type owl:Restriction ;
                                                                                          owl:onProperty <http://purl.obolibrary.org/obo/RO_0001000> ;
                                                                                          owl:someValuesFrom <http://purl.obolibrary.org/obo/FOODON_00002613>
                                                                                        ]
                                                                                        [ rdf:type owl:Restriction ;
                                                                                          owl:onProperty <http://purl.obolibrary.org/obo/RO_0001000> ;
                                                                                          owl:allValuesFrom <http://purl.obolibrary.org/obo/FOODON_00002613>
                                                                                        ]
                                                                                      ) ;
                                                                   rdf:type owl:Class
                                                                 ] ;
                                                 <http://purl.obolibrary.org/obo/IAO_0000114> <http://purl.obolibrary.org/obo/IAO_0000122> ;
                                                 <http://purl.obolibrary.org/obo/IAO_0000115> "Syrah wine is a white wine produced entirely from Syrah grapes.  The wines are often powerfully flavoured and full-bodied."@en ;
                                                 <http://purl.obolibrary.org/obo/IAO_0000117> "Ginny Pichler" ;
                                                 <http://purl.obolibrary.org/obo/IAO_0000119> "https://en.wikipedia.org/wiki/Syrah#Shiraz_wines" ;
                                                 <http://schema.org/image> <https://upload.wikimedia.org/wikipedia/commons/thumb/8/8e/Walla_walla_Syrah.jpg/179px-Walla_walla_Syrah.jpg> ;
                                                 rdfs:label "Syrah wine"@en .


###  http://purl.obolibrary.org/obo/FOODON_00002613
<http://purl.obolibrary.org/obo/FOODON_00002613> rdf:type owl:Class ;
                                                 rdfs:subClassOf <http://purl.obolibrary.org/obo/FOODON_03412121> ;
                                                 <http://purl.obolibrary.org/obo/IAO_0000114> <http://purl.obolibrary.org/obo/IAO_0000122> ;
                                                 <http://purl.obolibrary.org/obo/IAO_0000115> "Syrah is a dark-skinned grape variety grown throughout the world and used primarily to produce red wine. In 1999, Syrah was found to be the offspring of two obscure grapes from southeastern France, Dureza and Mondeuse Blanche."@en ;
                                                 <http://purl.obolibrary.org/obo/IAO_0000117> "Ginny Pichler" ;
                                                 <http://purl.obolibrary.org/obo/IAO_0000119> "https://en.wikipedia.org/wiki/Syrah" ;
                                                 <http://schema.org/image> <https://upload.wikimedia.org/wikipedia/commons/thumb/e/eb/Shiraz_Grapes.jpg/320px-Shiraz_Grapes.jpg> ;
                                                 <http://www.geneontology.org/formats/oboInOwl#hasExactSynonym> "Shiraz"@en ;
                                                 rdfs:label "Syrah grape plant"@en .


###  http://purl.obolibrary.org/obo/FOODON_00002614
<http://purl.obolibrary.org/obo/FOODON_00002614> rdf:type owl:Class ;
                                                 rdfs:subClassOf <http://purl.obolibrary.org/obo/FOODON_03310272> ,
                                                                 [ owl:intersectionOf ( [ rdf:type owl:Restriction ;
                                                                                          owl:onProperty <http://purl.obolibrary.org/obo/RO_0001000> ;
                                                                                          owl:someValuesFrom <http://purl.obolibrary.org/obo/FOODON_00002615>
                                                                                        ]
                                                                                        [ rdf:type owl:Restriction ;
                                                                                          owl:onProperty <http://purl.obolibrary.org/obo/RO_0001000> ;
                                                                                          owl:allValuesFrom <http://purl.obolibrary.org/obo/FOODON_00002615>
                                                                                        ]
                                                                                      ) ;
                                                                   rdf:type owl:Class
                                                                 ] ;
                                                 <http://purl.obolibrary.org/obo/IAO_0000114> <http://purl.obolibrary.org/obo/IAO_0000122> ;
                                                 <http://purl.obolibrary.org/obo/IAO_0000115> "Tempranillo wine is a red wine varietal produced entirely from Tempranillo grapes."@en ;
                                                 <http://purl.obolibrary.org/obo/IAO_0000117> "Damion Dooley" ;
                                                 <http://purl.obolibrary.org/obo/IAO_0000119> "https://en.wikipedia.org/wiki/Tempranillo" ;
                                                 rdfs:label "Tempranillo wine"@en .


###  http://purl.obolibrary.org/obo/FOODON_00002615
<http://purl.obolibrary.org/obo/FOODON_00002615> rdf:type owl:Class ;
                                                 rdfs:subClassOf <http://purl.obolibrary.org/obo/FOODON_03412121> ;
                                                 <http://purl.obolibrary.org/obo/IAO_0000114> <http://purl.obolibrary.org/obo/IAO_0000122> ;
                                                 <http://purl.obolibrary.org/obo/IAO_0000115> "Tempranillo is a black grape variety widely grown to make full-bodied red wines in its native Spain."@en ;
                                                 <http://purl.obolibrary.org/obo/IAO_0000117> "Damion Dooley" ;
                                                 <http://purl.obolibrary.org/obo/IAO_0000119> "https://en.wikipedia.org/wiki/Tempranillo" ;
                                                 <http://www.geneontology.org/formats/oboInOwl#hasExactSynonym> "Aragonez"@pt ,
                                                                                                                "Cencibel"@es ,
                                                                                                                "Tinta Roriz"@pt ,
                                                                                                                "Tinta del Pais"@es ,
                                                                                                                "Ull de Llebre"@es ;
                                                 rdfs:label "Tempranillo grape plant"@en .


###  http://purl.obolibrary.org/obo/FOODON_00002617
<http://purl.obolibrary.org/obo/FOODON_00002617> rdf:type owl:Class ;
                                                 rdfs:subClassOf <http://purl.obolibrary.org/obo/FOODON_03310272> ,
                                                                 [ owl:intersectionOf ( [ rdf:type owl:Restriction ;
                                                                                          owl:onProperty <http://purl.obolibrary.org/obo/RO_0001000> ;
                                                                                          owl:someValuesFrom <http://purl.obolibrary.org/obo/FOODON_00002618>
                                                                                        ]
                                                                                        [ rdf:type owl:Restriction ;
                                                                                          owl:onProperty <http://purl.obolibrary.org/obo/RO_0001000> ;
                                                                                          owl:allValuesFrom <http://purl.obolibrary.org/obo/FOODON_00002618>
                                                                                        ]
                                                                                      ) ;
                                                                   rdf:type owl:Class
                                                                 ] ;
                                                 <http://purl.obolibrary.org/obo/IAO_0000114> <http://purl.obolibrary.org/obo/IAO_0000122> ;
                                                 <http://purl.obolibrary.org/obo/IAO_0000115> "Zinfandel wine is a red wine varietal produced entirely from Zinfandel grapes.  A classic wine is high in both alcohol and tannins, intensely flavored and deeply colored."@en ;
                                                 <http://purl.obolibrary.org/obo/IAO_0000117> "Ginny Pichler" ;
                                                 <http://purl.obolibrary.org/obo/IAO_0000119> "https://www.wine-searcher.com/grape-391-primitivo" ;
                                                 rdfs:label "Zinfandel wine"@en .


###  http://purl.obolibrary.org/obo/FOODON_00002618
<http://purl.obolibrary.org/obo/FOODON_00002618> rdf:type owl:Class ;
                                                 rdfs:subClassOf <http://purl.obolibrary.org/obo/FOODON_03412121> ;
                                                 <http://purl.obolibrary.org/obo/IAO_0000114> <http://purl.obolibrary.org/obo/IAO_0000122> ;
                                                 <http://purl.obolibrary.org/obo/IAO_0000115> "Zinfandel is a variety of black-skinned wine grape."@en ;
                                                 <http://purl.obolibrary.org/obo/IAO_0000117> "Ginny Pichler" ;
                                                 <http://purl.obolibrary.org/obo/IAO_0000119> "https://en.wikipedia.org/wiki/Zinfandel" ;
                                                 <http://schema.org/image> <https://upload.wikimedia.org/wikipedia/commons/f/fc/Zinfandel_grapes.jpg> ;
                                                 <http://www.geneontology.org/formats/oboInOwl#hasExactSynonym> "Primitivo"@en ;
                                                 rdfs:label "Zinfandel grape plant"@en .


###  http://purl.obolibrary.org/obo/FOODON_00002619
<http://purl.obolibrary.org/obo/FOODON_00002619> rdf:type owl:Class ;
                                                 rdfs:subClassOf <http://purl.obolibrary.org/obo/FOODON_03310272> ,
                                                                 [ owl:intersectionOf ( [ rdf:type owl:Restriction ;
                                                                                          owl:onProperty <http://purl.obolibrary.org/obo/RO_0001000> ;
                                                                                          owl:someValuesFrom <http://purl.obolibrary.org/obo/FOODON_00002620>
                                                                                        ]
                                                                                        [ rdf:type owl:Restriction ;
                                                                                          owl:onProperty <http://purl.obolibrary.org/obo/RO_0001000> ;
                                                                                          owl:allValuesFrom <http://purl.obolibrary.org/obo/FOODON_00002620>
                                                                                        ]
                                                                                      ) ;
                                                                   rdf:type owl:Class
                                                                 ] ;
                                                 <http://purl.obolibrary.org/obo/IAO_0000114> <http://purl.obolibrary.org/obo/IAO_0000122> ;
                                                 <http://purl.obolibrary.org/obo/IAO_0000115> "Frappato wine is a red wine varietal produced entirely from Frappato grapes.  As a varietal, Frappato produces light bodied wines with a distinct grapey aroma."@en ;
                                                 <http://purl.obolibrary.org/obo/IAO_0000117> "Damion Dooley" ;
                                                 <http://purl.obolibrary.org/obo/IAO_0000119> "https://en.wikipedia.org/wiki/Frappato" ;
                                                 <http://www.geneontology.org/formats/oboInOwl#hasExactSynonym> "Frappato Nero"@it ,
                                                                                                                "Frappato Nero di Vittoria"@it ,
                                                                                                                "Frappatu"@it ,
                                                                                                                "Frappatu di Vittoria"@it ,
                                                                                                                "Nerello"@it ,
                                                                                                                "Nerello di Catania"@it ,
                                                                                                                "Nero Capitano."@it ;
                                                 rdfs:label "Frappato wine"@en .


###  http://purl.obolibrary.org/obo/FOODON_00002620
<http://purl.obolibrary.org/obo/FOODON_00002620> rdf:type owl:Class ;
                                                 rdfs:subClassOf <http://purl.obolibrary.org/obo/FOODON_03412121> ;
                                                 <http://purl.obolibrary.org/obo/IAO_0000114> <http://purl.obolibrary.org/obo/IAO_0000122> ;
                                                 <http://purl.obolibrary.org/obo/IAO_0000115> "Frappato di Vittoria or Frappato is a red Italian wine grape variety planted primarily in Sicily."@en ;
                                                 <http://purl.obolibrary.org/obo/IAO_0000117> "Damion Dooley" ;
                                                 <http://purl.obolibrary.org/obo/IAO_0000119> "https://en.wikipedia.org/wiki/Frappato" ;
                                                 <http://www.geneontology.org/formats/oboInOwl#hasExactSynonym> "Frappato di Vittoria"@it ;
                                                 rdfs:label "Frappato grape plant"@en .


###  http://purl.obolibrary.org/obo/FOODON_00002621
<http://purl.obolibrary.org/obo/FOODON_00002621> rdf:type owl:Class ;
                                                 rdfs:subClassOf <http://purl.obolibrary.org/obo/FOODON_03310272> ,
                                                                 [ owl:intersectionOf ( [ rdf:type owl:Restriction ;
                                                                                          owl:onProperty <http://purl.obolibrary.org/obo/RO_0001000> ;
                                                                                          owl:someValuesFrom <http://purl.obolibrary.org/obo/FOODON_00002622>
                                                                                        ]
                                                                                        [ rdf:type owl:Restriction ;
                                                                                          owl:onProperty <http://purl.obolibrary.org/obo/RO_0001000> ;
                                                                                          owl:allValuesFrom <http://purl.obolibrary.org/obo/FOODON_00002622>
                                                                                        ]
                                                                                      ) ;
                                                                   rdf:type owl:Class
                                                                 ] ;
                                                 <http://purl.obolibrary.org/obo/IAO_0000114> <http://purl.obolibrary.org/obo/IAO_0000122> ;
                                                 <http://purl.obolibrary.org/obo/IAO_0000115> "Gamay noir wine is a red wine varietal produced entirely from Gamay grapes."@en ;
                                                 <http://purl.obolibrary.org/obo/IAO_0000117> "Damion Dooley" ;
                                                 <http://purl.obolibrary.org/obo/IAO_0000119> "https://en.wikipedia.org/wiki/Gamay" ;
                                                 rdfs:label "Gamay noir wine"@en .


###  http://purl.obolibrary.org/obo/FOODON_00002622
<http://purl.obolibrary.org/obo/FOODON_00002622> rdf:type owl:Class ;
                                                 rdfs:subClassOf <http://purl.obolibrary.org/obo/FOODON_03412121> ;
                                                 <http://purl.obolibrary.org/obo/IAO_0000114> <http://purl.obolibrary.org/obo/IAO_0000122> ;
                                                 <http://purl.obolibrary.org/obo/IAO_0000115> "Gamay is a purple-colored grape variety used to make red wines, most notably grown in Beaujolais and in the Loire Valley around Tours."@en ;
                                                 <http://purl.obolibrary.org/obo/IAO_0000117> "Damion Dooley" ;
                                                 <http://purl.obolibrary.org/obo/IAO_0000119> "https://en.wikipedia.org/wiki/Gamay" ;
                                                 <http://schema.org/image> <https://upload.wikimedia.org/wikipedia/commons/3/38/Gamay.jpg> ;
                                                 <http://www.geneontology.org/formats/oboInOwl#hasExactSynonym> "Gamay Noir à Jus Blanc"@fr ;
                                                 rdfs:label "Gamay grape plant"@en .


###  http://purl.obolibrary.org/obo/FOODON_00002623
<http://purl.obolibrary.org/obo/FOODON_00002623> rdf:type owl:Class ;
                                                 rdfs:subClassOf <http://purl.obolibrary.org/obo/FOODON_03310273> ,
                                                                 [ owl:intersectionOf ( [ rdf:type owl:Restriction ;
                                                                                          owl:onProperty <http://purl.obolibrary.org/obo/RO_0001000> ;
                                                                                          owl:someValuesFrom <http://purl.obolibrary.org/obo/FOODON_00002624>
                                                                                        ]
                                                                                        [ rdf:type owl:Restriction ;
                                                                                          owl:onProperty <http://purl.obolibrary.org/obo/RO_0001000> ;
                                                                                          owl:allValuesFrom <http://purl.obolibrary.org/obo/FOODON_00002624>
                                                                                        ]
                                                                                      ) ;
                                                                   rdf:type owl:Class
                                                                 ] ;
                                                 <http://purl.obolibrary.org/obo/IAO_0000114> <http://purl.obolibrary.org/obo/IAO_0000122> ;
                                                 <http://purl.obolibrary.org/obo/IAO_0000115> "Gewürztraminerwine is a white wine varietal produced entirely from Gewürztraminer grapes."@en ;
                                                 <http://purl.obolibrary.org/obo/IAO_0000117> "Damion Dooley" ;
                                                 <http://purl.obolibrary.org/obo/IAO_0000119> "https://en.wikipedia.org/wiki/Gew%C3%BCrztraminer" ;
                                                 rdfs:label "Gewürztraminer wine"@en .


###  http://purl.obolibrary.org/obo/FOODON_00002624
<http://purl.obolibrary.org/obo/FOODON_00002624> rdf:type owl:Class ;
                                                 rdfs:subClassOf <http://purl.obolibrary.org/obo/FOODON_03412121> ;
                                                 <http://purl.obolibrary.org/obo/IAO_0000114> <http://purl.obolibrary.org/obo/IAO_0000122> ;
                                                 <http://purl.obolibrary.org/obo/IAO_0000115> "Gewürztraminer is an aromatic wine grape variety, used in white wines, and performs best in cooler climates."@en ;
                                                 <http://purl.obolibrary.org/obo/IAO_0000117> "Damion Dooley" ;
                                                 <http://purl.obolibrary.org/obo/IAO_0000119> "https://en.wikipedia.org/wiki/Gew%C3%BCrztraminer" ;
                                                 <http://schema.org/image> <https://upload.wikimedia.org/wikipedia/en/thumb/1/11/Gewurztraminer_-_raisins_sur_pied_de_vigne.jpg/320px-Gewurztraminer_-_raisins_sur_pied_de_vigne.jpg> ;
                                                 <http://www.geneontology.org/formats/oboInOwl#hasExactSynonym> "Gewurztraminer"@fr ,
                                                                                                                "Gewürz"@en ;
                                                 rdfs:label "Gewürztraminer grape plant"@en .


###  http://purl.obolibrary.org/obo/FOODON_00002625
<http://purl.obolibrary.org/obo/FOODON_00002625> rdf:type owl:Class ;
                                                 rdfs:subClassOf <http://purl.obolibrary.org/obo/FOODON_03310272> ,
                                                                 [ owl:intersectionOf ( [ rdf:type owl:Restriction ;
                                                                                          owl:onProperty <http://purl.obolibrary.org/obo/RO_0001000> ;
                                                                                          owl:someValuesFrom <http://purl.obolibrary.org/obo/FOODON_00002626>
                                                                                        ]
                                                                                        [ rdf:type owl:Restriction ;
                                                                                          owl:onProperty <http://purl.obolibrary.org/obo/RO_0001000> ;
                                                                                          owl:allValuesFrom <http://purl.obolibrary.org/obo/FOODON_00002626>
                                                                                        ]
                                                                                      ) ;
                                                                   rdf:type owl:Class
                                                                 ] ;
                                                 <http://purl.obolibrary.org/obo/IAO_0000114> <http://purl.obolibrary.org/obo/IAO_0000122> ;
                                                 <http://purl.obolibrary.org/obo/IAO_0000115> "Carignane wine is a red wine varietal produced entirely from Carignane grapes."@en ;
                                                 <http://purl.obolibrary.org/obo/IAO_0000117> "Damion Dooley" ;
                                                 <http://purl.obolibrary.org/obo/IAO_0000119> "https://en.wikipedia.org/wiki/Carignan" ;
                                                 rdfs:label "Carignane wine"@en .


###  http://purl.obolibrary.org/obo/FOODON_00002626
<http://purl.obolibrary.org/obo/FOODON_00002626> rdf:type owl:Class ;
                                                 rdfs:subClassOf <http://purl.obolibrary.org/obo/FOODON_03412121> ;
                                                 <http://purl.obolibrary.org/obo/IAO_0000114> <http://purl.obolibrary.org/obo/IAO_0000122> ;
                                                 <http://purl.obolibrary.org/obo/IAO_0000115> "Carignan (also known as Carignane) is a red grape variety of Spanish origin that is more commonly found in French wine but is widely planted throughout the western Mediterranean and around the globe."@en ;
                                                 <http://purl.obolibrary.org/obo/IAO_0000117> "Damion Dooley" ;
                                                 <http://purl.obolibrary.org/obo/IAO_0000119> "https://en.wikipedia.org/wiki/Carignan" ;
                                                 <http://schema.org/image> <https://upload.wikimedia.org/wikipedia/commons/thumb/7/77/Carignan_Viala_et_Vermorel.jpg/415px-Carignan_Viala_et_Vermorel.jpg> ;
                                                 <http://www.geneontology.org/formats/oboInOwl#hasExactSynonym> "Bovale Grande"@it ,
                                                                                                                "Carignano"@it ,
                                                                                                                "Carinyena"@es ,
                                                                                                                "Cariñena"@es ,
                                                                                                                "Mazuelo"@es ,
                                                                                                                "Samsó"@es ;
                                                 rdfs:label "Carignane grape plant"@en .


###  http://purl.obolibrary.org/obo/FOODON_00002627
<http://purl.obolibrary.org/obo/FOODON_00002627> rdf:type owl:Class ;
                                                 rdfs:subClassOf <http://purl.obolibrary.org/obo/FOODON_03310272> ,
                                                                 [ owl:intersectionOf ( [ rdf:type owl:Restriction ;
                                                                                          owl:onProperty <http://purl.obolibrary.org/obo/RO_0001000> ;
                                                                                          owl:someValuesFrom <http://purl.obolibrary.org/obo/FOODON_00002628>
                                                                                        ]
                                                                                        [ rdf:type owl:Restriction ;
                                                                                          owl:onProperty <http://purl.obolibrary.org/obo/RO_0001000> ;
                                                                                          owl:allValuesFrom <http://purl.obolibrary.org/obo/FOODON_00002628>
                                                                                        ]
                                                                                      ) ;
                                                                   rdf:type owl:Class
                                                                 ] ;
                                                 <http://purl.obolibrary.org/obo/IAO_0000114> <http://purl.obolibrary.org/obo/IAO_0000122> ;
                                                 <http://purl.obolibrary.org/obo/IAO_0000115> "Grenache wine is a red wine varietal produced entirely from Grenache grapes."@en ;
                                                 <http://purl.obolibrary.org/obo/IAO_0000117> "Damion Dooley" ;
                                                 <http://purl.obolibrary.org/obo/IAO_0000119> "https://en.wikipedia.org/wiki/Grenache" ;
                                                 rdfs:label "Grenache wine"@en .


###  http://purl.obolibrary.org/obo/FOODON_00002628
<http://purl.obolibrary.org/obo/FOODON_00002628> rdf:type owl:Class ;
                                                 rdfs:subClassOf <http://purl.obolibrary.org/obo/FOODON_03412121> ;
                                                 <http://purl.obolibrary.org/obo/IAO_0000114> <http://purl.obolibrary.org/obo/IAO_0000122> ;
                                                 <http://purl.obolibrary.org/obo/IAO_0000115> "Grenache is one of the most widely planted red wine grape varieties in the world."@en ;
                                                 <http://purl.obolibrary.org/obo/IAO_0000117> "Damion Dooley" ;
                                                 <http://purl.obolibrary.org/obo/IAO_0000119> "https://en.wikipedia.org/wiki/Grenache" ;
                                                 <http://schema.org/image> <https://upload.wikimedia.org/wikipedia/commons/thumb/b/bd/Grenache_N.jpg/440px-Grenache_N.jpg> ;
                                                 <http://www.geneontology.org/formats/oboInOwl#hasExactSynonym> "Garnacha"@es ;
                                                 rdfs:label "Grenache grape plant"@en .


###  http://purl.obolibrary.org/obo/FOODON_00002629
<http://purl.obolibrary.org/obo/FOODON_00002629> rdf:type owl:Class ;
                                                 rdfs:subClassOf <http://purl.obolibrary.org/obo/FOODON_03310272> ,
                                                                 [ owl:intersectionOf ( [ rdf:type owl:Restriction ;
                                                                                          owl:onProperty <http://purl.obolibrary.org/obo/RO_0001000> ;
                                                                                          owl:someValuesFrom <http://purl.obolibrary.org/obo/FOODON_00002630>
                                                                                        ]
                                                                                        [ rdf:type owl:Restriction ;
                                                                                          owl:onProperty <http://purl.obolibrary.org/obo/RO_0001000> ;
                                                                                          owl:allValuesFrom <http://purl.obolibrary.org/obo/FOODON_00002630>
                                                                                        ]
                                                                                      ) ;
                                                                   rdf:type owl:Class
                                                                 ] ;
                                                 <http://purl.obolibrary.org/obo/IAO_0000114> <http://purl.obolibrary.org/obo/IAO_0000122> ;
                                                 <http://purl.obolibrary.org/obo/IAO_0000115> "Barbera wine is a red wine varietal produced entirely from Barbera grapes."@en ;
                                                 <http://purl.obolibrary.org/obo/IAO_0000117> "Damion Dooley" ;
                                                 <http://purl.obolibrary.org/obo/IAO_0000119> "https://en.wikipedia.org/wiki/Barbera" ;
                                                 rdfs:label "Barbera wine"@en .


###  http://purl.obolibrary.org/obo/FOODON_00002630
<http://purl.obolibrary.org/obo/FOODON_00002630> rdf:type owl:Class ;
                                                 rdfs:subClassOf <http://purl.obolibrary.org/obo/FOODON_03412121> ;
                                                 <http://purl.obolibrary.org/obo/IAO_0000114> <http://purl.obolibrary.org/obo/IAO_0000122> ;
                                                 <http://purl.obolibrary.org/obo/IAO_0000115> "Barbera is a red Italian wine grape variety that, as of 2000, was the third most-planted red grape variety in Italy (after Sangiovese and Montepulciano). It produces good yields and is known for deep color, full body, low tannins and high levels of acid."@en ;
                                                 <http://purl.obolibrary.org/obo/IAO_0000117> "Damion Dooley" ;
                                                 <http://purl.obolibrary.org/obo/IAO_0000119> "https://en.wikipedia.org/wiki/Barbera" ;
                                                 <http://schema.org/image> <https://upload.wikimedia.org/wikipedia/commons/2/25/Barbera_cluster.JPG> ;
                                                 rdfs:label "Barbera grape plant"@en .

[ rdf:type owl:Axiom ;
   owl:annotatedSource <http://purl.obolibrary.org/obo/FOODON_00002630> ;
   owl:annotatedProperty <http://schema.org/image> ;
   owl:annotatedTarget <https://upload.wikimedia.org/wikipedia/commons/2/25/Barbera_cluster.JPG> ;
   <http://purl.org/dc/elements/1.1/date> "Agne27"@en ;
   <http://purl.org/dc/elements/1.1/license> <https://creativecommons.org/licenses/by-sa/3.0>
 ] .


###  http://purl.obolibrary.org/obo/FOODON_00002639
<http://purl.obolibrary.org/obo/FOODON_00002639> rdf:type owl:Class ;
                                                 rdfs:subClassOf <http://purl.obolibrary.org/obo/FOODON_00002577> ;
                                                 <http://purl.obolibrary.org/obo/IAO_0000114> <http://purl.obolibrary.org/obo/IAO_0000122> ;
                                                 <http://purl.obolibrary.org/obo/IAO_0000115> "Zakynthos Wine is wine produced on the Greek island of Zakynthos (Zante) in the Ionian Sea. A wide array of native Ionian grape varieties have been planted on the island for centuries, and are most famously used to make the intensely flavored, highly acidic Verdea wine."@en ;
                                                 <http://purl.obolibrary.org/obo/IAO_0000117> "Damion Dooley" ;
                                                 <http://purl.obolibrary.org/obo/IAO_0000119> "https://www.wine-searcher.com/regions-zakynthos" ;
                                                 <http://www.geneontology.org/formats/oboInOwl#hasExactSynonym> "zante wine"@en ;
                                                 rdfs:label "Zakynthos Wine"@en .


###  http://purl.obolibrary.org/obo/FOODON_00002640
<http://purl.obolibrary.org/obo/FOODON_00002640> rdf:type owl:Class ;
                                                 rdfs:subClassOf <http://purl.obolibrary.org/obo/FOODON_03412121> ;
                                                 <http://purl.obolibrary.org/obo/IAO_0000114> <http://purl.obolibrary.org/obo/IAO_0000122> ;
                                                 <http://purl.obolibrary.org/obo/IAO_0000115> "The Cabernet Sauvignon grape plant originates from a cross between Cabernet Franc and Sauvignon blanc varieties. It produces Cabernet Sauvignon grapes, a red wine grape variety."@en ;
                                                 <http://purl.obolibrary.org/obo/IAO_0000117> "Emma Griffiths" ;
                                                 <http://purl.obolibrary.org/obo/IAO_0000119> "https://en.wikipedia.org/wiki/Cabernet_Sauvignon" ;
                                                 <http://schema.org/image> <https://upload.wikimedia.org/wikipedia/commons/3/32/Red_Mountain_Cabernet_Sauvignon_grapes_from_Hedge_Vineyards.jpg> ;
                                                 rdfs:label "Cabernet Sauvignon grape plant"@en .

[ rdf:type owl:Axiom ;
   owl:annotatedSource <http://purl.obolibrary.org/obo/FOODON_00002640> ;
   owl:annotatedProperty <http://schema.org/image> ;
   owl:annotatedTarget <https://upload.wikimedia.org/wikipedia/commons/3/32/Red_Mountain_Cabernet_Sauvignon_grapes_from_Hedge_Vineyards.jpg> ;
   <http://purl.org/dc/terms/license> <http://creativecommons.org/licenses/by-sa/3.0/> ;
   <http://purl.org/dc/terms/rightsHolder> "Agne27 at the English Wikipedia"
 ] .


###  http://purl.obolibrary.org/obo/FOODON_00002641
<http://purl.obolibrary.org/obo/FOODON_00002641> rdf:type owl:Class ;
                                                 rdfs:subClassOf <http://purl.obolibrary.org/obo/FOODON_00002577> ;
                                                 <http://purl.obolibrary.org/obo/IAO_0000114> <http://purl.obolibrary.org/obo/IAO_0000122> ;
                                                 <http://purl.obolibrary.org/obo/IAO_0000115> "A Bordeaux wine is any wine produced in the Bordeaux region of southwest France."@en ;
                                                 <http://purl.obolibrary.org/obo/IAO_0000117> "Damion Dooley" ;
                                                 <http://purl.obolibrary.org/obo/IAO_0000119> "https://en.wikipedia.org/wiki/Bordeaux_wine" ;
                                                 <http://www.geneontology.org/formats/oboInOwl#hasExactSynonym> "claret"@en-br ;
                                                 rdfs:label "Bordeaux wine"@en .


###  http://purl.obolibrary.org/obo/FOODON_00002863
<http://purl.obolibrary.org/obo/FOODON_00002863> rdf:type owl:Class ;
                                                 rdfs:subClassOf <http://purl.obolibrary.org/obo/FOODON_03412121> ;
                                                 <http://purl.obolibrary.org/obo/IAO_0000114> <http://purl.obolibrary.org/obo/IAO_0000122> ;
                                                 <http://purl.obolibrary.org/obo/IAO_0000115> "Blaufränkisch (German for blue Frankish) is a dark-skinned variety of grape used for red wine."@en ;
                                                 <http://purl.obolibrary.org/obo/IAO_0000117> "Damion Dooley" ;
                                                 <http://purl.obolibrary.org/obo/IAO_0000119> "https://en.wikipedia.org/wiki/Blaufr%C3%A4nkisch" ;
                                                 <http://www.geneontology.org/formats/oboInOwl#hasExactSynonym> "Blauer Limberger"@ge ,
                                                                                                                "Blaufränkisch grape"@ge ,
                                                                                                                "Blue Limberger"@ge ,
                                                                                                                "lemberger"@ge ;
                                                 rdfs:label "Blaufränkisch grape plant"@en .


###  http://purl.obolibrary.org/obo/FOODON_00002864
<http://purl.obolibrary.org/obo/FOODON_00002864> rdf:type owl:Class ;
                                                 rdfs:subClassOf <http://purl.obolibrary.org/obo/FOODON_03310272> ,
                                                                 [ owl:intersectionOf ( [ rdf:type owl:Restriction ;
                                                                                          owl:onProperty <http://purl.obolibrary.org/obo/RO_0001000> ;
                                                                                          owl:someValuesFrom <http://purl.obolibrary.org/obo/FOODON_00002863>
                                                                                        ]
                                                                                        [ rdf:type owl:Restriction ;
                                                                                          owl:onProperty <http://purl.obolibrary.org/obo/RO_0001000> ;
                                                                                          owl:allValuesFrom <http://purl.obolibrary.org/obo/FOODON_00002863>
                                                                                        ]
                                                                                      ) ;
                                                                   rdf:type owl:Class
                                                                 ] ;
                                                 <http://purl.obolibrary.org/obo/IAO_0000114> <http://purl.obolibrary.org/obo/IAO_0000122> ;
                                                 <http://purl.obolibrary.org/obo/IAO_0000115> "Blaufränkisch wine is a red wine varietal produced entirely from Blaufränkisch grapes."@en ;
                                                 <http://purl.obolibrary.org/obo/IAO_0000117> "Damion Dooley" ;
                                                 <http://purl.obolibrary.org/obo/IAO_0000119> "https://en.wikipedia.org/wiki/Blaufr%C3%A4nkisch" ;
                                                 rdfs:label "Blaufränkisch wine"@en .


###  http://purl.obolibrary.org/obo/FOODON_00002868
<http://purl.obolibrary.org/obo/FOODON_00002868> rdf:type owl:Class ;
                                                 rdfs:subClassOf <http://purl.obolibrary.org/obo/FOODON_03412121> ;
                                                 <http://purl.obolibrary.org/obo/IAO_0000114> <http://purl.obolibrary.org/obo/IAO_0000122> ;
                                                 <http://purl.obolibrary.org/obo/IAO_0000115> "Mourvèdre (also known as Mataró or Monastrell) is a red wine grape variety that is grown in many regions around the world including the Rhône and Provence regions of France, the Valencia and Jumilla denominaciones de origen of Spain, as well as the Balearic Islands, California and Washington and the Australian regions of South Australia and New South Wales, as well as South Africa."@en ;
                                                 <http://purl.obolibrary.org/obo/IAO_0000117> "Damion Dooley" ;
                                                 <http://purl.obolibrary.org/obo/IAO_0000119> "https://en.wikipedia.org/wiki/Mourv%C3%A8dre" ;
                                                 <http://schema.org/image> <https://upload.wikimedia.org/wikipedia/commons/thumb/c/c6/Balzac_noir-mourvedre.jpg/451px-Balzac_noir-mourvedre.jpg> ;
                                                 <http://www.geneontology.org/formats/oboInOwl#hasExactSynonym> "Monastrell"@es ,
                                                                                                                "Mourvèdre grape | Mataró | Monastrell"@en ;
                                                 rdfs:label "Mourvèdre grape plant"@en .


###  http://purl.obolibrary.org/obo/FOODON_00002869
<http://purl.obolibrary.org/obo/FOODON_00002869> rdf:type owl:Class ;
                                                 rdfs:subClassOf <http://purl.obolibrary.org/obo/FOODON_03310272> ,
                                                                 [ owl:intersectionOf ( [ rdf:type owl:Restriction ;
                                                                                          owl:onProperty <http://purl.obolibrary.org/obo/RO_0001000> ;
                                                                                          owl:someValuesFrom <http://purl.obolibrary.org/obo/FOODON_00002868>
                                                                                        ]
                                                                                        [ rdf:type owl:Restriction ;
                                                                                          owl:onProperty <http://purl.obolibrary.org/obo/RO_0001000> ;
                                                                                          owl:allValuesFrom <http://purl.obolibrary.org/obo/FOODON_00002868>
                                                                                        ]
                                                                                      ) ;
                                                                   rdf:type owl:Class
                                                                 ] ;
                                                 <http://purl.obolibrary.org/obo/IAO_0000114> <http://purl.obolibrary.org/obo/IAO_0000122> ;
                                                 <http://purl.obolibrary.org/obo/IAO_0000117> "Damion Dooley" ;
                                                 <http://purl.obolibrary.org/obo/IAO_0000119> "https://en.wikipedia.org/wiki/Mourv%C3%A8dre" ;
                                                 rdfs:label "Mourvèdre wine"@en .


###  http://purl.obolibrary.org/obo/FOODON_03301014
<http://purl.obolibrary.org/obo/FOODON_03301014> rdf:type owl:Class ;
                                                 rdfs:label "grape wine"@en .


###  http://purl.obolibrary.org/obo/FOODON_03310272
<http://purl.obolibrary.org/obo/FOODON_03310272> rdf:type owl:Class ;
                                                 rdfs:label "red wine"@en .


###  http://purl.obolibrary.org/obo/FOODON_03310273
<http://purl.obolibrary.org/obo/FOODON_03310273> rdf:type owl:Class ;
                                                 rdfs:label "white wine"@en .


###  http://purl.obolibrary.org/obo/FOODON_03311123
<http://purl.obolibrary.org/obo/FOODON_03311123> rdf:type owl:Class ;
                                                 rdfs:subClassOf <http://purl.obolibrary.org/obo/FOODON_00002577> ;
                                                 <http://purl.obolibrary.org/obo/IAO_0000114> <http://purl.obolibrary.org/obo/IAO_0000122> ;
                                                 <http://purl.obolibrary.org/obo/IAO_0000115> "Chablis wine is a wine made in the Chablis region of France."@en ;
                                                 <http://purl.obolibrary.org/obo/IAO_0000117> "Emma Griffiths" ;
                                                 <http://purl.obolibrary.org/obo/IAO_0000119> "https://en.wikipedia.org/wiki/Chablis_wine" ;
                                                 rdfs:label "Chablis wine"@en .


###  http://purl.obolibrary.org/obo/FOODON_03311270
<http://purl.obolibrary.org/obo/FOODON_03311270> rdf:type owl:Class ;
                                                 rdfs:subClassOf <http://purl.obolibrary.org/obo/FOODON_00002577> ;
                                                 <http://purl.obolibrary.org/obo/IAO_0000114> <http://purl.obolibrary.org/obo/IAO_0000122> ;
                                                 <http://purl.obolibrary.org/obo/IAO_0000115> "Beaujolais is a French Appellation d'Origine Contrôlée (AOC) wine generally made of the Gamay grape which has a thin skin and is low in tannins."@en ;
                                                 <http://purl.obolibrary.org/obo/IAO_0000117> "Damion Dooley" ;
                                                 <http://purl.obolibrary.org/obo/IAO_0000119> "https://en.wikipedia.org/wiki/Beaujolais" ;
                                                 <http://schema.org/image> <https://upload.wikimedia.org/wikipedia/commons/thumb/d/d8/Carte_vignoble_beaujolais.png/356px-Carte_vignoble_beaujolais.png> ;
                                                 rdfs:label "Beaujolais wine"@en .


###  http://purl.obolibrary.org/obo/FOODON_03411329
<http://purl.obolibrary.org/obo/FOODON_03411329> rdf:type owl:Class ;
                                                 rdfs:label "grape plant"@en .


###  http://purl.obolibrary.org/obo/FOODON_03412121
<http://purl.obolibrary.org/obo/FOODON_03412121> rdf:type owl:Class ;
                                                 rdfs:label "european grape plant"@en .


###  Generated by the OWL API (version 5.1.14) https://github.com/owlcs/owlapi/
